Sorting/MergeSort.v
@@ -68,23 +68,76 @@ match goal with
         simpl in H; inversion_clear H
 end.
 
-Function hms (n : nat) (A : LinDec) (l : list A) {measure length l}
-  : list A :=
+Function hms (n : nat) (A : LinDec) (sort : list A -> list A) (l : list A)
+  {measure length l} : list A :=
   if @leqb natle (length l) (S (S n))
-  then insertionSort A l
+  then sort l
   else  let n := Nat.div2 (length l) in
         let l1 := take n l in
         let l2 := drop n l in
-          merge A (hms n A l1, hms n A l2).
+          merge A (hms n A sort l1, hms n A sort l2).
+Proof.
+  all: auto.
+Defined. 
+
+(* Parametrized mergesort *)
+Function hms2 (n : nat) (A : LinDec) (sort : list A -> list A) (l : list A)
+  {measure length l} : list A :=
+  if @leqb natle (length l) (S (S n))
+  then sort l
+  else let (l1, l2) := ms_split l in
+    merge A (hms2 n A sort l1, hms2 n A sort l2).
 Proof.
   all: auto.
 Defined.
 
-Function hms2 (n : nat) (A : LinDec) (l : list A) {measure length l}
-  : list A :=
-  if @leqb natle (length l) (S (S n))
-  then insertionSort A l
-  else let (l1, l2) := ms_split l in merge A (hms2 n A l1, hms2 n A l2).
+Class Split (A : Type) : Type :=
+{
+    split' : list A -> list A * list A;
+    spec1 : forall l l1 l2 : list A,
+        split' l = (l1, l2) -> 2 <= length l -> length l1 < length l;
+    spec2 : forall l l1 l2 : list A,
+        split' l = (l1, l2) -> 2 <= length l -> length l2 < length l;
+}.
+
+Coercion split' : Split >-> Funclass.
+
+Function ghms (n : nat) (A : LinDec)
+  (sort : list A -> list A) (split : Split A)
+  (l : list A) {measure length l} : list A :=
+    if @leqb natle (length l) (S (S n))
+    then sort l
+    else let (l1, l2) := split l in
+      merge A (ghms n A sort split l1, ghms n A sort split l2).
 Proof.
-  all: auto.
+  intros. apply spec2 with l1.
+    assumption.
+    destruct (@leqb_spec natle (length l) (S (S n))); cbn in *.
+      congruence.
+      omega.
+  intros. apply spec1 with l2.
+    assumption.
+    destruct (@leqb_spec natle (length l) (S (S n))); cbn in *.
+      congruence.
+      omega.
 Defined.
+
+Instance MsSplit (A : LinDec) : Split A :=
+{
+    split' := ms_split
+}.
+Proof.
+  intros. destruct l as [| x [| y t]]; cbn in *.
+    omega.
+    omega.
+    eapply ms_split_len1. eauto.
+  intros. destruct l as [| x [| y t]]; cbn in *.
+    omega.
+    omega.
+    eapply ms_split_len2. eauto.
+Defined.
+
+Definition wut (A : LinDec) (l : list A) : list A :=
+  ghms 0 A (fun l => l) (MsSplit A) l.
+
+Compute wut natle testl.
