Sorting/Heapsort.v
@@ -1,0 +1,38 @@
+Add Rec LoadPath "/home/zeimer/Code/Coq".
+
+Require Export Coq.Program.Wf.
+Require Export Recdef.
+
+Require Export Sorting.Sort.
+Require Export ListLemmas.
+
+Require Export BTree.
+Require Export BST.
+Require Export LeftistHeap.
+
+Set Implicit Arguments.
+
+(* Leftist heapsort *)
+Function fromList {A : LinDec} (l : list A) : BTree A :=
+match l with
+    | [] => emptyHeap
+    | h :: t => insert' h (fromList t)
+end.
+
+Function toList {A : LinDec} (t : BTree A)
+  {measure len t} : list A :=
+match deleteMin t with
+    | (None, _) => []
+    | (Some m, t') => m :: toList t'
+end.
+Proof.
+  destruct t; cbn; inversion 1; inversion 1; subst.
+  rewrite merge'_len. omega.
+Defined.
+
+Arguments toList [x] _.
+
+Definition leftistHeapsort (A : LinDec) (l : list A)
+  : list A := toList (fromList l).
+
+Time Compute leftistHeapsort natle (cycle 25 testl).
