Sorting/HeapsortSpec.v
@@ -1,0 +1,95 @@
+Add Rec LoadPath "/home/zeimer/Code/Coq".
+
+Require Export Coq.Program.Wf.
+Require Export Recdef.
+
+Require Export Sorting.Sort.
+Require Export ListLemmas.
+
+Require Export BTree.
+Require Export BST.
+Require Export LeftistHeap.
+
+Require Export Heapsort.
+
+Set Implicit Arguments.
+
+Lemma toList_sorted :
+  forall (A : LinDec) (t : BTree A),
+    is_heap t -> sorted A (toList t).
+Proof.
+  intros A t. functional induction @toList A t.
+    constructor.
+    functional induction @toList A t'; constructor.
+      eapply deleteMin_spec; eauto. eapply deleteMin_elem. eauto.
+      apply IHl. eapply deleteMin_is_heap; eauto.
+Qed.
+
+Lemma fromList_is_heap :
+  forall (A : LinDec) (l : list A),
+    is_heap (fromList l).
+Proof.
+  intros. functional induction @fromList A l; cbn.
+    constructor.
+    unfold insert'. apply merge'_is_heap; auto.
+      constructor; auto; inversion 1.
+Qed.
+
+Theorem leftistHeapsort_sorted :
+  forall (A : LinDec) (l : list A),
+    sorted A (leftistHeapsort A l).
+Proof.
+  unfold leftistHeapsort. intros.
+    apply toList_sorted. apply fromList_is_heap.
+Qed.
+
+Lemma count_BTree_merge' :
+  forall (A : LinDec) (x : A) (t1 t2 : BTree A),
+    count_BTree A x (merge' (t1, t2)) =
+    count_BTree A x t1 + count_BTree A x t2.
+Proof.
+  intros. remember (t1, t2) as p.
+  functional induction @merge' A p; inv Heqp; clear Heqp;
+  balance; cbn; rewrite (IHb _ _ _ eq_refl); dec.
+Qed.
+
+Lemma count_BTree_insert :
+  forall (A : LinDec) (x y : A) (t : BTree A),
+    count_BTree A x (insert' y t) =
+      if x =? y
+      then S (count_BTree A x t)
+      else count_BTree A x t.
+Proof.
+  intros. unfold insert'. rewrite count_BTree_merge'. dec.
+Qed.
+
+Lemma count_fromList :
+  forall (A : LinDec) (x : A) (l : list A),
+    count_BTree A x (fromList l) = count A x l.
+Proof.
+  intros. functional induction @fromList A l;
+  try rewrite count_BTree_insert; dec.
+Qed.
+
+Lemma count_toList :
+  forall (A : LinDec) (x : A) (t : BTree A),
+    count A x (toList t) = count_BTree A x t.
+Proof.
+  intros. functional induction @toList A t; cbn;
+  destruct t; inv e; dec; rewrite IHl, count_BTree_merge'; trivial.
+Qed.
+
+Theorem leftistHeapsort_perm :
+  forall (A : LinDec) (l : list A),
+    perm A l (leftistHeapsort A l).
+Proof.
+  unfold perm, leftistHeapsort. intros.
+  rewrite count_toList, count_fromList. trivial.
+Qed.
+
+Instance Sort_leftistHeapsort : Sort :=
+{
+    sort := @leftistHeapsort;
+    sort_sorted := @leftistHeapsort_sorted;
+    sort_perm := leftistHeapsort_perm
+}.
