Sorting/TrichQuicksort.v
@@ -1,0 +1,82 @@
+Add Rec LoadPath "/home/zeimer/Code/Coq".
+
+Require Export Coq.Program.Wf.
+Require Export Recdef.
+
+Require Export Sorting.Sort.
+Require Export ListLemmas.
+
+Require Import TrichDec.
+
+Set Implicit Arguments.
+
+Local Hint Unfold lt.
+Local Hint Resolve le_n_S filter_length.
+
+Function htqs (n : nat) (A : TrichDec) (sort : list A -> list A) (l : list A)
+  {measure length l} : list A :=
+if @trichb_ltb natlt (length l) (S n)
+then sort l
+else match l with
+    | [] => []
+    | h :: t =>
+        let '(lo, eq, hi) := trifilter' h t in
+          htqs n A sort lo ++ h :: eq ++ htqs n A sort hi
+end.
+Proof.
+  intros. rewrite trifilter'_spec in teq1. inversion teq1; subst; cbn.
+    pose (filter_length (fun x => h <? x) t). omega.
+  intros. rewrite trifilter'_spec in teq1. inversion teq1; subst; cbn.
+    pose (filter_length (fun x => x <? h) t). omega.
+Defined.
+
+Definition tqs (A : TrichDec) (l : list A) : list A :=
+  htqs 0 A (fun l => l) l.
+
+Class Partition (A : Type) : Type :=
+{
+    partition :> A -> list A -> list A * list A * list A;
+    spec_lo : forall (h : A) (t l1 l2 l3 : list A),
+      partition h t = (l1, l2, l3) -> length l1 <= length t;
+    spec_hi : forall (h : A) (t l1 l2 l3 : list A),
+      partition h t = (l1, l2, l3) -> length l3 <= length t
+}.
+
+Coercion partition : Partition >-> Funclass.
+
+Function htqs2
+  (n : nat) (A : TrichDec)
+  (sort : list A -> list A) (partition : Partition A)
+  (l : list A) {measure length l} : list A :=
+    if @trichb_ltb natlt (length l) (S n)
+    then sort l
+    else match l with
+        | [] => []
+        | h :: t =>
+            let '(lo, eq, hi) := partition h t in
+              htqs2 n A sort partition lo ++
+              h :: eq ++
+              htqs2 n A sort partition hi
+    end.
+Proof.
+  intros. apply spec_hi in teq1. cbn. omega.
+  intros. apply spec_lo in teq1. cbn. omega.
+Defined.
+
+Instance Trifilter (A : TrichDec) : Partition A :=
+{
+    partition := trifilter'
+}.
+Proof.
+  intros. rewrite trifilter'_spec in H. inversion H; subst; cbn.
+    apply filter_length.
+  intros. rewrite trifilter'_spec in H. inversion H; subst; cbn.
+    apply filter_length.
+Defined.
+
+Definition wut (A : TrichDec) (l : list A) : list A :=
+  htqs2 0 A (fun l => l) (Trifilter A) l.
+
+Time Compute wut natlt (cycle 30 testl).
+Time Compute tqs natlt (cycle 3000 testl).
+Time Compute tqs natlt (cycle 1500 [1]).
