Trees/LeftistHeap2.v
@@ -1,0 +1,394 @@
+Add Rec LoadPath "/home/zeimer/Code/Coq".
+
+Require Export LinDec.
+Require Import Sorting.Sort.
+
+Set Implicit Arguments.
+
+Inductive RSTree (A : Type) : Type :=
+    | empty : RSTree A
+    | node : nat -> A -> RSTree A -> RSTree A -> RSTree A.
+
+Arguments empty [A].
+Arguments node [A] _ _ _.
+
+Definition right_spine {A : Type} (t : RSTree A) : nat :=
+match t with
+    | empty => 0
+    | node n _ _ _ => n
+end.
+
+Inductive elem {A : Type} (x : A) : RSTree A -> Prop :=
+    | elem_root : forall (n : nat) (l r : RSTree A),
+        elem x (node n x l r)
+    | elem_left : forall (n : nat) (v : A) (l r : RSTree A),
+        elem x l -> elem x (node n v l r)
+    | elem_right : forall  (n : nat) (v : A) (l r : RSTree A),
+        elem x r -> elem x (node n v l r).
+
+Inductive is_heap {A : LinDec} : RSTree A -> Prop :=
+    | is_heap_empty : is_heap empty
+    | is_heap_node :
+        forall  (n : nat) (v : A) (l : RSTree A) (r : RSTree A),
+          (forall x : A, elem x l -> v ≤ x) -> is_heap l ->
+          (forall x : A, elem x r -> v ≤ x) -> is_heap r ->
+            is_heap (node n v l r).
+
+Lemma is_heap_inv_l :
+  forall (A : LinDec) (n : nat) (v : A) (l r : RSTree A),
+    is_heap (node n v l r) -> is_heap l.
+Proof.
+  inversion 1; eauto.
+Qed.
+
+Lemma is_heap_inv_r :
+  forall (A : LinDec) (n : nat) (v : A) (l r : RSTree A),
+    is_heap (node n v l r) -> is_heap r.
+Proof.
+  inversion 1; eauto.
+Qed.
+
+Lemma is_heap_inv_leq :
+  forall (A : LinDec) (n : nat) (v : A) (l r : RSTree A),
+    is_heap (node n v l r) -> forall x : A,
+      elem x (node n v l r) -> v ≤ x.
+Proof.
+  do 2 inversion 1; subst; auto.
+Qed.
+
+Hint Resolve is_heap_inv_l is_heap_inv_r.
+
+Inductive left_biased {A : LinDec} : RSTree A -> Prop :=
+    | left_biased_empty : left_biased empty
+    | left_biased_node :
+        forall (v : A) (l r : RSTree A),
+          right_spine r <= right_spine l ->
+          left_biased l -> left_biased r ->
+            left_biased (node (S (right_spine r)) v l r).
+
+Hint Constructors RSTree elem is_heap left_biased.
+
+Ltac lh x :=
+  let t := fresh "t" in
+  let H := fresh "H" in
+  let H' := fresh "H" in
+    destruct x as [t H H']; destruct t;
+    try inversion H; try inversion H'; subst; cbn.
+
+Ltac inv x := inversion x; subst; auto.
+
+Definition getMin {A : LinDec} (t : RSTree A) : option A :=
+match t with
+    | empty => None
+    | node _ v _ _ => Some v
+end.
+
+(*Theorem getMin_spec :
+  forall (A : LinDec) (h : LeftistHeap A) (m : A),
+    getMin h = Some m -> forall x : A, elem x h -> m ≤ x.
+Proof.
+  lh h; inversion 1; subst. inversion 1; auto.
+Qed.
+
+Definition emptyHeap {A : LinDec} : LeftistHeap A.
+Proof.
+  split with (tree := empty); auto.
+Defined.
+
+Theorem emptyHeap_spec :
+  forall (A : LinDec) (x : A), ~ elem x emptyHeap.
+Proof.
+  inversion 1.
+Qed.*)
+
+Definition singleton' {A : Type} (x : A)
+  : RSTree A := node 1 x empty empty.
+
+(*Definition singleton {A : LinDec} (x : A) : LeftistHeap A.
+Proof.
+  split with (tree := singleton' x);
+  constructor; auto; inversion 1.
+Defined.*)
+
+Ltac elem :=
+  intros; unfold singleton' in *; cbn in *; subst; repeat
+match goal with
+    | |- elem ?x (node ?x _ _) => constructor
+    | H : elem _ empty |- _ => inv H
+    | H : elem _ (node _ empty empty) |- _ => inv H
+    | H : elem _ _ /\ elem _ _ |- _ => destruct H
+    | H : elem _ _ \/ elem _ _ |- _ => destruct H
+end; auto.
+
+(*Theorem singleton_spec :
+  forall (A : LinDec) (x y : A),
+    elem x (singleton y) <-> x = y.
+Proof.
+  split; elem.
+Qed.*)
+
+Definition balance {A : Type} (v : A) (l r : RSTree A) : RSTree A :=
+  if right_spine r <=? right_spine l
+  then node (S (right_spine r)) v l r
+  else node (S (right_spine l)) v r l.
+
+Ltac balance := unfold balance in *;
+match goal with
+    | H : context [right_spine ?r <=? right_spine ?l] |- _ =>
+        destruct (@leqb_spec natle (right_spine r) (right_spine l))
+    | |- context [right_spine ?r <=? right_spine ?l] =>
+        destruct (@leqb_spec natle (right_spine r) (right_spine l))
+end.
+
+Fixpoint size {A : Type} (t : RSTree A) : nat :=
+match t with
+    | empty => 0
+    | node _ _ l r => S (size l + size r)
+end.
+
+Lemma size_swap :
+  forall (A : Type) (n : nat) (v : A) (l r : RSTree A),
+    size (node n v r l) = size (node n v l r).
+Proof.
+  intros. cbn. omega.
+Qed.
+
+Lemma balance_size:
+  forall (A : Type) (n : nat) (v : A) (l r : RSTree A),
+    size (balance v l r) = size (node n v l r).
+Proof.
+  intros. balance.
+    trivial.
+    cbn. omega.
+Qed.
+
+Lemma balance_elem :
+  forall (A : Type) (n : nat) (x v : A) (l r : RSTree A),
+    elem x (balance v l r) <-> elem x (node n v l r).
+Proof.
+  intros. balance; split; intro; inv H.
+Qed.
+
+Theorem balance_is_heap :
+  forall (A : LinDec) (n : nat) (v : A) (l r : RSTree A),
+    (forall x : A, elem x l -> v ≤ x) ->
+    (forall x : A, elem x r -> v ≤ x) ->
+      is_heap l -> is_heap r -> is_heap (balance v l r).
+Proof.
+  intros; balance; constructor; elem.
+Qed.
+
+Theorem balance_left_biased :
+  forall (A : LinDec) (n : nat) (v : A) (l r : RSTree A),
+    left_biased l -> left_biased r ->
+      left_biased (balance v l r).
+Proof.
+  intros. balance; constructor; cbn in *; dec.
+Qed.
+
+Require Import Recdef.
+
+Definition sum_of_sizes {A : Type} (p : RSTree A * RSTree A) : nat :=
+  size (fst p) + size (snd p).
+
+Function merge' {A : LinDec} (p : RSTree A * RSTree A)
+  {measure sum_of_sizes p} : RSTree A :=
+match p with
+    | (empty, t2) => t2
+    | (t1, empty) => t1
+    | (node _ v l r as t1, node _ v' l' r' as t2) =>
+        if v <=? v'
+        then balance v l (merge' (r, t2))
+        else balance v' l' (merge' (t1, r'))
+end.
+Proof.
+  1-2: intros; cbn; omega.
+Defined.
+
+Arguments merge' [x] _.
+
+Lemma elem_merge' :
+  forall (A : LinDec) (x : A) (t1 t2 : RSTree A),
+    elem x (merge' (t1, t2)) -> elem x t1 \/ elem x t2.
+Proof.
+  intros. remember (t1, t2) as p.
+  functional induction @merge' A p; inv Heqp; clear Heqp; auto.
+    rewrite balance_elem in H. inv H. edestruct IHr; eauto.
+    rewrite balance_elem in H. inv H. edestruct IHr; eauto.
+    Unshelve. all: auto.
+Qed.
+
+Lemma elem_merge'_v2 :
+  forall (A : LinDec) (x : A) (t1 t2 : RSTree A),
+    elem x t1 \/ elem x t2 -> elem x (merge' (t1, t2)).
+Proof.
+  intros. remember (t1, t2) as p.
+  functional induction @merge' A p; inv Heqp; clear Heqp;
+  elem; rewrite balance_elem.
+    inv H. apply elem_right.
+      eapply IHr; try ((left + right); eauto); reflexivity.
+    apply elem_right.
+      eapply IHr; try ((left + right); eauto); reflexivity.
+    apply elem_right.
+      eapply IHr; try ((left + right); eauto); reflexivity.
+    inv H. apply elem_right.
+      eapply IHr; try ((left + right); eauto); reflexivity.
+    Unshelve. all: auto.
+Qed.
+
+Theorem merge'_spec :
+  forall (A : LinDec) (x : A) (t1 t2 : RSTree A),
+    elem x (merge' (t1, t2)) <-> elem x t1 \/ elem x t2.
+Proof.
+  split; intros. elem.
+    apply elem_merge'. assumption.
+    apply elem_merge'_v2. assumption.
+Qed.
+
+Arguments elem_merge' [A x t1 t2] _.
+
+Theorem merge'_size:
+  forall (A : LinDec) (t1 t2 : RSTree A),
+    size (merge' (t1, t2)) = size t1 + size t2.
+Proof.
+  intros. remember (t1, t2) as p.
+  functional induction @merge' A p; inv Heqp; clear Heqp.
+    erewrite balance_size. cbn. rewrite (IHr r (node _ v' l' r') eq_refl).
+      cbn. omega.
+    erewrite balance_size. cbn. rewrite (IHr (node _ v l r) r' eq_refl).
+      cbn. omega.
+    Unshelve. all: auto.
+Qed.
+
+Theorem merge'_is_heap :
+  forall (A : LinDec) (t1 t2 : RSTree A),
+    is_heap t1 -> is_heap t2 -> is_heap (merge' (t1, t2)).
+Proof.
+  intros. remember (t1, t2) as p.
+  functional induction @merge' A p; inv Heqp; clear Heqp;
+  inv H; inv H0; apply balance_is_heap; elem.
+    destruct (leqb_spec v v'); inv e0. destruct (elem_merge' H1); auto.
+      eapply leq_trans with v'. auto. inv H2.
+    apply (IHr _ _ H8 H0 eq_refl).
+    destruct (leqb_spec v v'), (elem_merge' H1); inv e0.
+      eapply leq_trans with v. dec. inv H2.
+    apply (IHr _ _ H H12 eq_refl).
+Qed.
+
+Theorem merge'_left_biased :
+  forall (A : LinDec) (t1 t2 : RSTree A),
+    left_biased t1 -> left_biased t2 -> left_biased (merge' (t1, t2)).
+Proof.
+  intros. remember (t1, t2) as p.
+  functional induction @merge' A p; inv Heqp; clear Heqp;
+  inv H; inv H0; cbn in *; apply balance_left_biased; auto.
+    exact 0.
+    apply (IHr _ _ H7 H0 eq_refl).
+    exact 0.
+    apply (IHr _ _ H H10 eq_refl).
+Qed.
+
+(*Definition merge {A : LinDec} (h1 h2 : LeftistHeap A)
+  : LeftistHeap A.
+Proof.
+  destruct h1 as [t1 H11 H12], h2 as [t2 H21 H22].
+  split with (tree := @merge' A (t1, t2)).
+  apply merge'_is_heap; assumption.
+  apply merge'_left_biased; assumption.
+Defined.*)
+
+Definition insert' {A : LinDec} (x : A) (t : RSTree A) : RSTree A :=
+  merge' ((singleton' x), t).
+
+(* TODO *)
+(*Definition insert {A : LinDec} (x : A) (h : LeftistHeap A)
+  : LeftistHeap A.
+Proof.
+  split with (tree := merge (singleton x) h).
+    destruct (merge _ _). cbn. assumption.
+    destruct (merge _ _). cbn. assumption.
+Defined.
+
+Theorem insert_spec :
+  forall (A : LinDec) (x y : A) (h : LeftistHeap A),
+    elem x (insert y h) <-> x = y \/ elem x h.
+Proof.
+  split; destruct h; subst; cbn; intros.
+    destruct (elem_merge' H); auto. inv H0; inv H2.
+    destruct H; subst; apply elem_merge'_v2; elem.
+Qed.*)
+
+Definition deleteMin {A : LinDec} (t : RSTree A)
+  : option A * RSTree A :=
+match t with
+    | empty => (None, empty)
+    | node _ v l r => (Some v, merge' (l, r))
+end.
+
+Theorem deleteMin_spec :
+  forall (A : LinDec) (m : A) (t t' : RSTree A),
+    is_heap t -> deleteMin t = (Some m, t') ->
+      forall x : A, elem x t' -> m ≤ x.
+Proof.
+  destruct t; cbn; inversion 1; inversion 1; subst; cbn.
+  intros. destruct (elem_merge' H0); auto.
+Qed.
+
+Theorem deleteMin_size:
+  forall (A : LinDec) (m : A) (t t' : RSTree A),
+    deleteMin t = (Some m, t') -> size t = S (size t').
+Proof.
+  destruct t; cbn; inversion 1; subst. rewrite merge'_size. trivial.
+Qed.
+
+Theorem deleteMin_elem :
+  forall (A : LinDec) (m : A) (t t' : RSTree A),
+    deleteMin t = (Some m, t') -> elem m t.
+Proof.
+  destruct t; cbn; inversion 1. constructor.
+Qed.
+
+Theorem deleteMin_is_heap :
+  forall (A : LinDec) (m : A) (t t' : RSTree A),
+    is_heap t -> deleteMin t = (Some m, t') ->
+      is_heap t'.
+Proof.
+  destruct t; cbn; inversion 1; inversion 1; subst.
+  apply merge'_is_heap; assumption.
+Qed.
+
+Theorem deleteMin_left_biased :
+  forall (A : LinDec) (m : A) (t t' : RSTree A),
+    left_biased t -> deleteMin t = (Some m, t') ->
+      left_biased t'.
+Proof.
+  destruct t; cbn; do 2 inversion 1; subst.
+  apply merge'_left_biased; assumption.
+Qed.
+
+(* Leftist heapsort *)
+Function fromList {A : LinDec} (l : list A) : RSTree A :=
+match l with
+    | [] => empty
+    | h :: t => insert' h (fromList t)
+end.
+
+Function toList {A : LinDec} (t : RSTree A)
+  {measure size t} : list A :=
+match deleteMin t with
+    | (None, _) => []
+    | (Some m, t') => m :: toList t'
+end.
+Proof.
+  destruct t; cbn; inversion 1; inversion 1; subst.
+  rewrite merge'_size. omega.
+Defined.
+
+Arguments toList [x] _.
+
+Definition leftistHeapsort (A : LinDec) (l : list A)
+  : list A := toList (fromList l).
+
+Require Import ListLemmas.
+
+Time Compute leftistHeapsort natle (cycle 25 testl).
